theories/simplang/proofmode.v
@@ -118,7 +118,7 @@ Proof.
   iIntros "H". iApply source_red_bind. by iApply Hs.
 Qed.
 
-Lemma tac_target_red_allocN n v j i K Ψ Δ :
+Lemma tac_target_red_allocN n v j i K Ψ Δ `{!sheapInvConst} :
   (0 < n)%Z →
   (∀ l,
     match envs_app false (Esnoc (Esnoc Enil i († l …t Z.to_nat n)) j (l ↦t∗ (replicate (Z.to_nat n) v))) Δ with
@@ -136,7 +136,7 @@ Proof.
   rewrite envs_app_sound //; simpl. iApply "He"; iSplitL "Hl"; eauto.
 Qed.
 
-Lemma tac_source_red_allocN n v j i K Ψ Δ :
+Lemma tac_source_red_allocN n v j i K Ψ Δ `{!sheapInvConst}:
   (0 < n)%Z →
   (∀ l,
     match envs_app false (Esnoc (Esnoc Enil i (†l …s Z.to_nat n)) j (l ↦s∗ (replicate (Z.to_nat n) v))) Δ with
@@ -154,7 +154,7 @@ Proof.
   iApply HΔ. rewrite envs_app_sound //; simpl. iApply "He"; iSplitL "Hl"; eauto.
 Qed.
 
-Lemma tac_target_red_alloc v j i K Ψ Δ :
+Lemma tac_target_red_alloc v j i K Ψ Δ `{!sheapInvConst}:
   (∀ l,
     match envs_app false (Esnoc (Esnoc Enil i (†l …t 1)) j (l ↦t v)) Δ with
     | Some Δ' =>
@@ -171,7 +171,7 @@ Proof.
   iApply HΔ. rewrite envs_app_sound //; simpl. iApply "He"; iSplitL "Hl"; eauto.
 Qed.
 
-Lemma tac_source_red_alloc v j i K Ψ Δ :
+Lemma tac_source_red_alloc v j i K Ψ Δ `{!sheapInvConst}:
   (∀ l,
     match envs_app false (Esnoc (Esnoc Enil i (†l …s 1)) j (l ↦s v)) Δ with
     | Some Δ' =>
@@ -188,7 +188,7 @@ Proof.
   iApply HΔ. rewrite envs_app_sound //; simpl. iApply "He"; iSplitL "Hl"; eauto.
 Qed.
 
-Lemma tac_target_red_free l v i j K Ψ Δ Δ' :
+Lemma tac_target_red_free l v i j K Ψ Δ Δ' `{!sheapInvConst}:
   envs_lookup_delete false i Δ = Some (false, l ↦t v, Δ')%I →
   envs_lookup j Δ' = Some (false, †l …t 1)%I →
   (let Δ'' := envs_delete false j false Δ' in
@@ -205,7 +205,7 @@ Proof.
   by iApply target_red_base.
 Qed.
 
-Lemma tac_source_red_free l v i j K Ψ Δ Δ' :
+Lemma tac_source_red_free l v i j K Ψ Δ Δ' `{!sheapInvConst}:
   envs_lookup_delete false i Δ = Some (false, l ↦s v, Δ')%I →
   envs_lookup j Δ' = Some (false, †l …s 1)%I →
   (let Δ'' := envs_delete false j false Δ' in
@@ -222,7 +222,7 @@ Proof.
   by iApply source_red_base.
 Qed.
 
-Lemma tac_target_red_freeN l (n : Z) vs i j K Ψ Δ Δ' :
+Lemma tac_target_red_freeN l (n : Z) vs i j K Ψ Δ Δ' `{!sheapInvConst}:
   n = length vs →
   envs_lookup_delete false i Δ = Some (false, l ↦t∗ vs, Δ')%I →
   envs_lookup j Δ' = Some (false, †l …t Z.to_nat n)%I →
@@ -240,7 +240,7 @@ Proof.
   by iApply target_red_base.
 Qed.
 
-Lemma tac_source_red_freeN l (n : Z) vs i j K Ψ Δ Δ' :
+Lemma tac_source_red_freeN l (n : Z) vs i j K Ψ Δ Δ' `{!sheapInvConst}:
   n = length vs →
   envs_lookup_delete false i Δ = Some (false, l ↦s∗ vs, Δ')%I →
   envs_lookup j Δ' = Some (false, †l …s Z.to_nat n)%I →
@@ -258,7 +258,7 @@ Proof.
   by iApply source_red_base.
 Qed.
 
-Lemma tac_target_red_loadsc Δ i K b l q v Ψ :
+Lemma tac_target_red_loadsc Δ i K b l q v Ψ `{!sheapInvConst}:
   envs_lookup i Δ = Some (b, l ↦t{#q} v)%I →
   envs_entails Δ (target_red (fill K (Val v)) Ψ) →
   envs_entails Δ (target_red (fill K (Load ScOrd (LitV l))) Ψ).
@@ -272,7 +272,7 @@ Proof.
   * apply sep_mono_r, wand_mono; first done. rewrite Hi. iIntros "Ht".
     iApply target_red_base; eauto.
 Qed.
-Lemma tac_target_red_loadna Δ i K b l v Ψ q:
+Lemma tac_target_red_loadna Δ i K b l v Ψ q `{!sheapInvConst}:
   envs_lookup i Δ = Some (b, l ↦t{#q} v)%I →
   envs_entails Δ (target_red (fill K (Val v)) Ψ) →
   envs_entails Δ (target_red (fill K (Load Na1Ord (LitV l))) Ψ).
@@ -287,7 +287,7 @@ Proof.
     iApply target_red_base; eauto.
 Qed.
 
-Lemma tac_source_red_loadsc Δ i K b l q v Ψ :
+Lemma tac_source_red_loadsc Δ i K b l q v Ψ `{!sheapInvConst}:
   envs_lookup i Δ = Some (b, l ↦s{#q} v)%I →
   envs_entails Δ (source_red (fill K (Val v)) π Ψ) →
   envs_entails Δ (source_red (fill K (Load ScOrd (LitV l))) π Ψ).
@@ -301,7 +301,7 @@ Proof.
   * apply sep_mono_r, wand_mono; first done. rewrite Hi. iIntros "Hs".
     iApply source_red_base; eauto.
 Qed.
-Lemma tac_source_red_loadna Δ i K b l v Ψ q:
+Lemma tac_source_red_loadna Δ i K b l v Ψ q `{!sheapInvConst}:
   envs_lookup i Δ = Some (b, l ↦s{#q} v)%I →
   envs_entails Δ (source_red (fill K (Val v)) π Ψ) →
   envs_entails Δ (source_red (fill K (Load Na1Ord (LitV l))) π Ψ).
@@ -317,13 +317,13 @@ Proof.
 Qed.
 
 
-Lemma target_red_store l v v' o Ψ :
+Lemma target_red_store l v v' o Ψ `{!sheapInvConst}:
   o = ScOrd ∨ o = Na1Ord →
   l ↦t v' -∗
   (l ↦t v -∗ target_red (of_val #()) Ψ) -∗
   target_red (Store o (Val $ LitV (LitLoc l)) (Val v)) Ψ.
 Proof. intros [-> | ->]; [iApply target_red_store_sc | iApply target_red_store_na]. Qed.
-Lemma tac_target_red_store Δ i K l v v' o Ψ :
+Lemma tac_target_red_store Δ i K l v v' o Ψ `{!sheapInvConst}:
   o = ScOrd ∨ o = Na1Ord →
   envs_lookup i Δ = Some (false, l ↦t v)%I →
   match envs_simple_replace i false (Esnoc Enil i (l ↦t v')) Δ with
@@ -340,13 +340,13 @@ Proof.
   rewrite Hi. iIntros "Ht". iApply target_red_base; eauto.
 Qed.
 
-Lemma source_red_store l v v' o Ψ :
+Lemma source_red_store l v v' o Ψ `{!sheapInvConst}:
   o = ScOrd ∨ o = Na1Ord →
   l ↦s v' -∗
   (l ↦s v -∗ source_red (of_val #()) π Ψ) -∗
   source_red (Store o (Val $ LitV (LitLoc l)) (Val v)) π Ψ.
 Proof. intros [-> | ->]; [iApply source_red_store_sc | iApply source_red_store_na]. Qed.
-Lemma tac_source_red_store Δ i K l v v' o Ψ :
+Lemma tac_source_red_store Δ i K l v v' o Ψ `{!sheapInvConst}:
   o = ScOrd ∨ o = Na1Ord →
   envs_lookup i Δ = Some (false, l ↦s v)%I →
   match envs_simple_replace i false (Esnoc Enil i (l ↦s v')) Δ with
@@ -976,13 +976,13 @@ Tactic Notation "source_free" :=
   | |- envs_entails _ (source_red ?e ?π ?Ψ) =>
     let process_single _ :=
       first
-        [reshape_expr e ltac:(fun K e' => eapply (tac_source_red_free _ _ _ _ _ K _ _ _))
+        [reshape_expr e ltac:(fun K e' => eapply (tac_source_red_free _ _ _ _ _ K Ψ _ _))
         |fail 1 "source_free: cannot find 'Free' in" e];
       [solve_mapsto () | solve_perm () | pm_reduce; source_finish]
     in
     let process_array _ :=
       first
-        [reshape_expr e ltac:(fun K e' => eapply (tac_source_red_freeN _ _ _ _ _ _ K _ _ _))
+        [reshape_expr e ltac:(fun K e' => eapply (tac_source_red_freeN _ _ _ _ _ _ K Ψ _ _))
         |fail 1 "source_free: cannot find 'FreeN' in" e];
       [idtac| solve_mapstoN () | solve_perm () | pm_reduce; source_finish]
     in (process_single ()) || (process_array ())
@@ -998,11 +998,11 @@ Tactic Notation "target_load" :=
   lazymatch goal with
   | |- envs_entails _ (target_red ?e ?Ψ) =>
     first
-      [reshape_expr e ltac:(fun K e' => eapply (tac_target_red_loadsc _ _ K _ _ _ _ _))
-      |reshape_expr e ltac:(fun K e' => eapply (tac_target_red_loadna _ _ K _ _ _ _))
+      [reshape_expr e ltac:(fun K e' => eapply (tac_target_red_loadsc _ _ K _ _ _ _ Ψ))
+      |reshape_expr e ltac:(fun K e' => eapply (tac_target_red_loadna _ _ K _ _ _ Ψ _))
       |fail 1 "target_load: cannot find 'Load' in" e];
     [ solve_mapsto ()
-    |target_finish]
+    | target_finish]
   | _ => fail "target_load: not a 'target_red'"
   end.
 
@@ -1015,11 +1015,11 @@ Tactic Notation "source_load" :=
   lazymatch goal with
   | |- envs_entails _ (source_red ?e ?π ?Ψ) =>
     first
-      [reshape_expr e ltac:(fun K e' => eapply (tac_source_red_loadsc _ _ _ K _ _ _ _ _))
-      |reshape_expr e ltac:(fun K e' => eapply (tac_source_red_loadna _ _ _ K _ _ _ _))
+      [reshape_expr e ltac:(fun K e' => eapply (tac_source_red_loadsc _ _ _ K _ _ _ _ Ψ))
+      |reshape_expr e ltac:(fun K e' => eapply (tac_source_red_loadna _ _ _ K _ _ _ Ψ _))
       |fail 1 "source_load: cannot find 'Load' in" e];
     [ solve_mapsto ()
-    |source_finish]
+    | source_finish]
   | _ => fail "source_load: not a 'source_red'"
   end.
 
